Full test for ConnectionTable3 experiment

src/tls/experiments/ConnectionTable3.fst
@@ -2,121 +2,171 @@ module ConnectionTable3
 
 open FStar.Tactics
 open FStar.ReflexiveTransitiveClosure
-open FStar.Monotonic.DependentTable
+open FStar.Monotonic.DependentMap
 
 open FStar.HyperStack
 open FStar.HyperStack.ST
 
-module T = FStar.Monotonic.DependentTable
+module T = FStar.Monotonic.DependentMap
 module DM = FStar.DependentMap
 
 type connection_id = nat
 
 assume val client_hello: Type0
 
-assume val has_cookie: client_hello -> bool
-
 assume val cookie : Type0
+
+assume val has_cookie: client_hello -> bool
 
 assume val ch_cookie: ch:client_hello{has_cookie ch} -> cookie
 
 assume val matches: cookie -> client_hello -> Type0
 
 noeq
-type connection =  
+type connection =
+  | Init: connection
   | Sent_HRR: random:nat -> ch:client_hello -> connection
-  | Sent_ServerHello: random:nat -> ch:client_hello -> connection
-  | Complete: random:nat -> ch:client_hello -> connection
+  | Sent_ServerHello: random:nat -> ch:client_hello -> id1:connection_id -> connection
+  | Complete: random:nat -> ch:client_hello -> id1:connection_id -> connection
 
-let nonce_of = function
-  | Sent_HRR r _ | Sent_ServerHello r _ | Complete r _ -> r
-
-let is_retry = function
-  | Sent_HRR _ _ -> false
-  | Sent_ServerHello _ ch | Complete _ ch -> has_cookie ch
-
-let cookie_of (c:connection{is_retry c}) =
+let nonce_of (c:connection{~(Init? c)}) =
   match c with
-  | Sent_ServerHello _ ch | Complete _ ch -> ch_cookie ch
+  | Sent_HRR r _ | Sent_ServerHello r _ _ | Complete r _ _ -> r
+
+let ch_of (c:connection{~(Init? c)}) =
+  match c with
+  | Sent_HRR _ ch | Sent_ServerHello _ ch _ | Complete _ ch _ -> ch
+
+let cookie_of (c:connection{~(Init? c) /\ has_cookie (ch_of c)}) =
+  ch_cookie (ch_of c)
+
+let id0_of (c:connection{Sent_ServerHello? c \/ Complete? c}) =
+  match c with
+  | Sent_ServerHello _ _ id0 | Complete _ _ id0 -> id0
 
 let step (s1 s2:connection) : Type0 =
   match s1, s2 with
-  | Sent_ServerHello r ch, Complete r' ch' -> r == r' /\ ch == ch'
+  | Init, Sent_HRR _ _ -> True
+  | Init, Sent_ServerHello _ _ _ -> True
+  | Sent_ServerHello r ch id0, Complete r' ch' id0' -> r == r' /\ ch == ch' /\ id0 == id0'
   | _, _ -> False
 
-unfold
 let rel : Preorder.preorder connection = closure step
 
-type connection_table (rgn:erid) = 
-  T.t rgn connection_id (fun _ -> mmmref connection rel) (fun _ -> True) (fun _ r1 r2 -> r1 == r2) 
+assume val rgn:erid
 
-val inv: rgn:erid -> t:connection_table rgn -> h:mem -> Type0
-let inv rgn t h = 
-  let m = T.repr (sel h t) in
-  forall (id:connection_id).
-   Some? (DM.sel m id) ==>
-   (let c = Some?.v (DM.sel m id) in
-    is_retry (sel h c) ==>
-    (exists (id':connection_id).
-     Some? (DM.sel m id') /\
-     (let c' = Some?.v (DM.sel m id') in
-      token_p c' (fun h0 -> 
-        Sent_HRR? (sel h0 c') /\ 
-        nonce_of (sel h0 c') == nonce_of (sel h c) /\
-        cookie_of (sel h c) `matches` Sent_HRR?.ch (sel h0 c')))))
+let connection_ref (id:connection_id) = r:mmmref connection rel{frameOf r `extends` rgn}
 
-val test: rgn:erid -> ch1:client_hello -> ch2:client_hello{has_cookie ch2} 
-  -> ST (connection_table rgn)
+let minv (m:partial_dependent_map connection_id connection_ref) =
+  forall id1 id2.{:pattern (Some? (DM.sel m id1)); (Some? (DM.sel m id2))}
+    (id1 <> id2 /\ Some? (DM.sel m id1) /\ Some? (DM.sel m id2)) ==>
+    frameOf (Some?.v (DM.sel m id1)) `disjoint` frameOf (Some?.v (DM.sel m id2))
+
+type connection_table = T.t rgn connection_id connection_ref minv
+
+val connection_inv: 
+    m:T.imap connection_id connection_ref minv
+  -> c:connection
+  -> Type0
+let connection_inv m c =
+  match c with
+  | Sent_ServerHello r ch id0 | Complete r ch id0 ->
+    if has_cookie ch then
+      match T.sel m id0 with
+      | Some c' ->
+        token_p c' (fun h0 -> 
+          Sent_HRR? (sel h0 c') /\ 
+          nonce_of (sel h0 c') == r /\
+          ch_cookie ch `matches` Sent_HRR?.ch (sel h0 c'))
+      | _ -> False
+    else True
+  | _ -> True
+
+(*
+  Stateful invariant
+  It can't be attached to the table because it needs to dereferences connections
+*)
+val inv: t:connection_table -> h:mem -> Type0
+let inv t h = 
+  let m = sel h t in
+  forall (id:connection_id).{:pattern (T.defined t id h)}
+    T.defined t id h ==> connection_inv m (sel h (Some?.v (T.sel m id)))
+
+val alloc: unit -> ST (connection_table)
+  (requires fun _ -> witnessed (region_contains_pred rgn))
+  (ensures  fun h0 t h1 -> ralloc_post rgn T.empty h0 t h1)
+let alloc _ =
+  T.alloc ()
+
+val create: t:connection_table -> id:connection_id -> ST (connection_ref id)
+  (requires fun h0 -> h0 `contains` t /\ inv t h0 /\ ~(T.defined t id h0))
+  (ensures  fun h0 c h1 -> 
+    mods [Ref t] h0 h1 /\ 
+    h1 `contains` t /\ 
+    inv t h1 /\
+    T.defined t id h1 /\
+    sel h1 t == T.upd (sel h0 t) id c /\
+    ~(h0 `contains` c) /\
+    h1 `contains` c /\
+    sel h1 c == Init)
+let create t id =
+  let h0 = get () in
+  let p (id:connection_id{T.defined t id h0}) = frameOf (T.value_of t id h0) in
+  testify_forall_region_contains_pred #_ #p ();
+  let rgn1 = new_region rgn in
+  let c : mmmref connection rel = ralloc_mm rgn1 Init in
+  let h1 = get () in
+  assert (forall (id:connection_id). T.defined t id h0 ==> ~(c == T.value_of t id h0));
+  assert (inv t h1);
+  T.extend t id c;
+  assert (
+    let m0 = sel h0 t in
+    forall (id':connection_id).{:pattern (T.value_of t id' h0)}
+      (T.defined t id' h0 /\ ~(c == T.value_of t id' h0)) ==>
+      connection_inv m0 (sel h1 (T.value_of t id' h0)));
+  c
+
+(* Added a pattern; all alternatives I tried didn't work or were too cumbersome *)
+val token_functoriality
+  (#a:Type0) (#rel:Preorder.preorder a) (r:mreference a rel)
+  (p:mem_predicate{token_p r p}) (q:mem_predicate{forall (h:mem). p h ==> q h})
+  : Lemma (token_p r q)
+   [SMTPat (token_p r p); SMTPat (token_p r q)]
+let token_functoriality #a #rel r p q = 
+  token_functoriality r p q
+
+#set-options "--z3rlimit 40"
+
+(*
+   This tests the server side of a full handshake with mismatched parameters:
+
+   1. Allocate an empty connection table 
+   2. Create a first connection c1 with id = 1 (in Init state)
+   3. Receive a ClientHello ch1 with random 0 on c1. Transition c1 to Sent_HRR 0 ch1
+   4. Create a second connection c2 (in Init state)
+   5. Receive a ClientHello ch2 on c2 with a random and cookie extension matching ch1.
+      Transition c2 to Sent_ServerHello 0 ch2 1, with c1 as the matching initial connection 
+   6. Receive a ClientFinished on c2. Transition c2 to Complete 0 ch2 1
+*)
+val test: ch1:client_hello -> ch2:client_hello{has_cookie ch2} -> ST connection_table
   (requires fun _ -> witnessed (region_contains_pred rgn) /\
                   ch_cookie ch2 `matches` ch1)
-  (ensures  fun h0 t h1 -> h1 `contains` t /\ frameOf t == rgn /\ inv rgn t h1)
-let test rgn ch1 ch2 =
-  let t : connection_table rgn = T.alloc () in
-  let c1 : mmmref connection rel = ralloc_mm rgn (Sent_HRR 1 ch1) in
-  T.update t 1 c1;
-  let h1 = get() in
-  assert (inv rgn t h1);
-  let c2 : mmmref connection rel = ralloc_mm rgn (Sent_ServerHello 1 ch2) in
-  T.update t 2 c2;  
-  let h2 = get() in
-  let rhs (c:connection) = 
-    Sent_HRR? c /\ 
-    nonce_of c == 1 /\
-    ch_cookie ch2 `matches` Sent_HRR?.ch c
-  in
-  stable_on_closure step rhs ();
-  witness_p c1 (fun h -> rhs (sel h c1));
-  assert (token_p c1 (fun h -> rhs (sel h c1)));
-  assume (
-   let m = T.repr (sel h2 t) in
-   forall (id:connection_id).
-     Some? (DM.sel m id) ==>
-     (let c = Some?.v (DM.sel m id) in
-      is_retry (sel h2 c) ==>
-      (exists (id':connection_id).
-        Some? (DM.sel m id) /\
-        (let c' = Some?.v (DM.sel m id) in
-        token_p c' (fun h0 -> rhs (sel h0 c'))))));
-//  admit();
-  assert (
-  let m = T.repr (sel h2 t) in
-  forall (id:connection_id).
-   Some? (DM.sel m id) ==>
-   (let c = Some?.v (DM.sel m id) in
-    is_retry (sel h2 c) ==>
-     Some? (DM.sel m 1) /\
-     (let c' = Some?.v (DM.sel m 1) in
-      token_p c' (fun h -> rhs (sel h c1)))));
-  assume (
-    inv rgn t h2 <==>
-    (let m = T.repr (sel h2 t) in
-  forall (id:connection_id).
-   Some? (DM.sel m id) ==>
-   (let c = Some?.v (DM.sel m id) in
-    is_retry (sel h2 c) ==>
-    (exists (id':connection_id).
-     Some? (DM.sel m id') /\
-     (let c' = Some?.v (DM.sel m id') in
-      token_p c' (fun h0 -> rhs (sel h0 c')))))));
-  admit();
+  (ensures  fun h0 t h1 -> h1 `contains` t /\ inv t h1)
+let test ch1 ch2 =
+  let t = alloc () in
+  let c1 = create t 1 in
+  c1 := Sent_HRR 0 ch1;
+  let c2 = create t 2 in
+  c2 := Sent_ServerHello 0 ch2 1;
+  stable_on_closure (closure step) 
+    (fun c ->
+      Sent_HRR? c /\ 
+      nonce_of c == 0 /\
+      ch_cookie ch2 `matches` Sent_HRR?.ch c) ();
+  witness_p c1 
+    (fun h -> 
+      Sent_HRR? (sel h c1) /\ 
+      nonce_of (sel h c1) == 0 /\
+      ch_cookie ch2 `matches` Sent_HRR?.ch (sel h c1));
+  c2 := Complete 0 ch2 1;
   t
